src/dvspec/dafny/att_spec_proofs/inv.dfy
@@ -4,6 +4,7 @@ include "../specification/consensus.dfy"
 include "../specification/network.dfy"
 include "../specification/dvn.dfy"
 include "../att_spec_proofs/helper_sets_lemmas.dfy"
+include "../specification/dvc_spec_axioms.dfy"
 
 
 
@@ -16,6 +17,7 @@ module Att_Inv_With_Empty_Initial_Attestation_Slashing_DB
     import opened DVCNode_Spec
     import opened DV
     import opened Helper_Sets_Lemmas
+    import opened DVCNode_Spec_Axioms
 
 
     // For every pair (n1, n2) of honest nodes working for the same attestation duty, 
